SSA/Projects/SLLVM/Dialect/Base.lean
@@ -28,23 +28,41 @@ of (side-effecting) UB.
 
 /-! ### Dialect definition -/
 
+inductive SLLVMOp where
+  | arith (o : LLVM.Op)
+  | ptradd
+  | load (w : Nat)
+  | store (w : Nat)
+  | free
+  deriving DecidableEq, Lean.ToExpr
+
+inductive SLLVMTy where
+  | arith (t : LLVM.Ty)
+  | ptr
+  deriving DecidableEq, Lean.ToExpr
+
 def SLLVM : Dialect where
-  Op := LLVM.Op
-  Ty := LLVM.Ty
+  Op := SLLVMOp
+  Ty := SLLVMTy
   m := EffectM
 
 namespace SLLVM
 
+instance : TyDenote SLLVM.Ty where
+  toType
+  | .arith t => ⟦t⟧
+  | .ptr => SLLVM.Ptr
+
 instance : DecidableEq SLLVM.Op := by unfold SLLVM; infer_instance
 instance : DecidableEq SLLVM.Ty := by unfold SLLVM; infer_instance
-instance : ToString SLLVM.Op    := by unfold SLLVM; infer_instance
-instance : ToString SLLVM.Ty    := by unfold SLLVM; infer_instance
-instance : Repr SLLVM.Op        := by unfold SLLVM; infer_instance
-instance : Repr SLLVM.Ty        := by unfold SLLVM; infer_instance
 instance : Lean.ToExpr SLLVM.Op := by unfold SLLVM; infer_instance
 instance : Lean.ToExpr SLLVM.Ty := by unfold SLLVM; infer_instance
 
-instance : TyDenote SLLVM.Ty    := by unfold SLLVM; infer_instance
+-- instance : ToString SLLVM.Op    := by unfold SLLVM; infer_instance
+-- instance : ToString SLLVM.Ty    := by unfold SLLVM; infer_instance
+-- instance : Repr SLLVM.Op        := by unfold SLLVM; infer_instance
+-- instance : Repr SLLVM.Ty        := by unfold SLLVM; infer_instance
+
 instance : Monad SLLVM.m        := by unfold SLLVM; infer_instance
 instance : LawfulMonad SLLVM.m  := by unfold SLLVM; infer_instance
 
@@ -52,37 +70,182 @@ open Qq in instance : DialectToExpr SLLVM where
   toExprDialect := q(SLLVM)
   toExprM := q(Id.{0})
 
-@[match_pattern]
-abbrev Ty.bitvec : Nat → SLLVM.Ty :=
-  InstCombine.LLVM.Ty.bitvec
-
-@[simp_denote] theorem toType_bitvec : TyDenote.toType (Ty.bitvec w) = LLVM.IntW w := rfl
-
 @[simp, simp_denote]
 theorem m_eq : SLLVM.m α = EffectM α := by rfl
 
-end SLLVM
+/-! ### Aliasses -/
+section Alias
+open InstCombine.LLVM SLLVMOp
+
+@[match_pattern] nonrec abbrev Ty.arith : LLVM.Ty → SLLVM.Ty := .arith
+
+@[match_pattern] abbrev Ty.bitvec (w : Nat) : SLLVM.Ty := .arith (.bitvec w)
+@[match_pattern] abbrev Ty.ptr : SLLVM.Ty := .ptr
+
+@[match_pattern] nonrec abbrev Op.arith : LLVM.Op → SLLVM.Op := .arith
+
+@[match_pattern] nonrec abbrev Op.neg (w : Nat) : SLLVM.Op := arith <| Op.neg w
+@[match_pattern] nonrec abbrev Op.not (w : Nat) : SLLVM.Op := arith <| Op.not w
+@[match_pattern] nonrec abbrev Op.copy (w : Nat) : SLLVM.Op := arith <| Op.copy w
+@[match_pattern] nonrec abbrev Op.sext (w w' : Nat) : SLLVM.Op := arith <| Op.sext w w'
+@[match_pattern] nonrec abbrev Op.zext (w w' : Nat) (flag : LLVM.NonNegFlag := { }) : SLLVM.Op := arith <| Op.zext w w' flag
+@[match_pattern] nonrec abbrev Op.trunc (w w' : Nat) (flags : LLVM.NoWrapFlags := { }) : SLLVM.Op := arith <| Op.trunc w w' flags
+
+@[match_pattern] nonrec abbrev Op.and (w : Nat) : SLLVM.Op := arith <| Op.and w
+@[match_pattern] nonrec abbrev Op.or (w : Nat) (flag : LLVM.DisjointFlag := { }) : SLLVM.Op := arith <| Op.or w flag
+@[match_pattern] nonrec abbrev Op.xor (w : Nat) : SLLVM.Op := arith <| Op.xor w
+@[match_pattern] nonrec abbrev Op.shl (w : Nat) (flags : LLVM.NoWrapFlags := { }) : SLLVM.Op := arith <| Op.shl w flags
+@[match_pattern] nonrec abbrev Op.lshr (w : Nat) (flag : LLVM.ExactFlag := { }) : SLLVM.Op := arith <| Op.lshr w flag
+@[match_pattern] nonrec abbrev Op.ashr (w : Nat) (flag : LLVM.ExactFlag := { }) : SLLVM.Op := arith <| Op.ashr w flag
+@[match_pattern] nonrec abbrev Op.add (w : Nat) (flags : LLVM.NoWrapFlags := { }) : SLLVM.Op := arith <| Op.add w flags
+@[match_pattern] nonrec abbrev Op.mul (w : Nat) (flags : LLVM.NoWrapFlags := { }) : SLLVM.Op := arith <| Op.mul w flags
+@[match_pattern] nonrec abbrev Op.sub (w : Nat) (flags : LLVM.NoWrapFlags := { }) : SLLVM.Op := arith <| Op.sub w flags
+
+@[match_pattern] nonrec abbrev Op.icmp (c : LLVM.IntPred) (w : Nat) : SLLVM.Op := arith <| Op.icmp c w
+@[match_pattern] nonrec abbrev Op.const (w : Nat) (val : Int) : SLLVM.Op := arith <| Op.const w val
+@[match_pattern] nonrec abbrev Op.select (w : Nat) : SLLVM.Op := arith <| Op.select w
+
+@[match_pattern] nonrec abbrev Op.udiv (w : Nat) (flag : LLVM.ExactFlag := { }) : SLLVM.Op := arith <| Op.udiv w flag
+@[match_pattern] nonrec abbrev Op.sdiv (w : Nat) (flag : LLVM.ExactFlag := { }) : SLLVM.Op := arith <| Op.sdiv w flag
+@[match_pattern] nonrec abbrev Op.urem : Nat → SLLVM.Op := arith ∘ Op.urem
+@[match_pattern] nonrec abbrev Op.srem : Nat → SLLVM.Op := arith ∘ Op.srem
+
+
+@[simp, simp_denote] theorem toType_arith : toType (Ty.arith t) = toType t := rfl
+@[simp, simp_denote] theorem toType_bitvec : toType (Ty.bitvec w) = LLVM.IntW w := rfl
+
+end Alias
 
 /-! ### Signature -/
 
-open InstCombine.LLVM.Op in
+open SLLVM.Ty in
 /-- The signature of each operation is the same as in LLVM. -/
 instance : DialectSignature SLLVM where
-  signature op :=
-    { DialectSignature.signature (d := LLVM) op with
+  signature
+  | .arith op => SLLVM.Ty.arith <$> { DialectSignature.signature (d := LLVM) op with
         effectKind := match op with
-          | udiv .. | sdiv .. | urem .. | srem .. => .impure
+          | .udiv .. | .sdiv .. | .urem .. | .srem .. => .impure
           | _ => .pure
-    }
+      }
+  | .ptradd => { sig := [ptr, bitvec 64], regSig := [], returnTypes := [ptr], effectKind := .pure }
+  | .load w => { sig := [ptr], regSig := [], returnTypes := [bitvec w], effectKind := .impure }
+  | .store w => { sig := [ptr, bitvec w], regSig := [], returnTypes := [], effectKind := .impure }
+  | .free => { sig := [ptr], regSig := [], returnTypes := [], effectKind := .impure }
 
-open InstCombine.LLVM.Op in
+
+/-! ### argsToLLVM Helper -/
+section ArgsToLLVM
+
+def argsToLLVM {tys : List LLVM.Ty} :
+    HVector toType (Ty.arith <$> tys) → HVector toType tys :=
+  HVector.cast (by simp) (by simp)
+
+open Qq Lean Meta in
+partial def reduceArgsToLLVMAux : Meta.Simp.DSimproc := fun e => do
+  let_expr argsToLLVM tys xs := e
+    | return .continue
+  withTraceNode `LeanMLIR.Elab (fun _ => pure m!"Simplifying application of `argsToLLVM`: {e}") <| do
+    let ⟨_, ys⟩ ← go tys xs
+    return .visit ys
+where go (tys xs : Lean.Expr) : MetaM (Σ (tys : Q(List LLVM.Ty)), Q(HVector toType $tys)) :=
+  match_expr xs with
+  | HVector.nil _ _ =>
+      return ⟨_, q(HVector.nil)⟩
+  | HVector.cons _α _A tys t y ys => do
+      let t' ← mkFreshExprMVarQ q(LLVM.Ty)
+      let expected := mkApp (mkConst ``Ty.arith) t'
+      unless (← isDefEq t expected) do
+        trace[LeanMLIR.Elab] "{crossEmoji} Failed to unify:\n\t{t}\nwith:\n\t{expected}\
+          \n\nIn implicit argument of expression:\n\t{xs}"
+      let ⟨tys', ys⟩ ← go tys ys
+      return ⟨
+        q($t' :: $tys'),
+        mkAppN (.const ``HVector.cons [0, 0]) #[
+          q(LLVM.Ty), q(@toType LLVM.Ty _), tys', t', y, ys
+        ]⟩
+  | _ => do
+      trace[LeanMLIR.Elab] "{crossEmoji} Failed to decompose:\n\t{xs}\
+        \nExpected either `HVector.cons` or `HVector.nil`"
+      return ⟨tys, xs⟩
+
+-- simproc [simp, simp_denote] reduceArgsToLLVM (argsToLLVM (tys := no_index _) (
+simproc reduceArgsToLLVM (argsToLLVM (tys := no_index (?t :: ?ts)) (
+    .cons (α := no_index _) (f := no_index _) (a := no_index _) (as := no_index _) _ _)
+  ) :=
+  -- reduceArgsToLLVMAux
+  fun _ => return .continue
+
+
+theorem foo (x : ⟦Ty.arith t⟧) (xs : HVector toType (Ty.arith <$> ts)) :
+    argsToLLVM (tys := no_index (t :: ts)) (
+      .cons (α := no_index _) (f := no_index _) (a := no_index (Ty.arith t)) (as := no_index (Ty.arith <$> ts)) x xs)
+    = zs := by
+  sorry
+#discr_tree_simp_key foo
+
+open Lean Meta Elab Command DiscrTree Simp in
+elab "#discr_tree_simproc_key " k:ident : command => liftTermElabM <| do
+  let state := simprocDeclExt.getState (← getEnv)
+  if let some (some keys) := state.newEntries[k.getId]? then
+    Lean.logInfo (← keysAsPattern keys)
+  else
+    let n ← realizeGlobalConstNoOverloadWithInfo k
+    if let some (some keys) := state.newEntries[n]? then
+      Lean.logInfo (← keysAsPattern keys)
+    else
+      throwErrorAt k "not a simproc: {k}"
+
+#discr_tree_simproc_key reduceArgsToLLVM
+
+/-!
+NOTE: we aggresively unfold `⟦t⟧` when `t` is a concrete type, and in our proof
+goals `t` is always a concrete goal. That is why in `argsToLLVM_cons` we have to
+specify `x : LLVM.IntW w`. Recall that Lean does not perform higher-order
+unification, so if we instead said `x : ⟦t⟧`, Lean would not be able to
+figure out that `t` should be assigned to `bitvec w` to unify `⟦t⟧` with
+`LLVM.IntW w`, and instead would fail to apply the rewrite!
+-/
+
+end ArgsToLLVM
+
+open Op in
 instance : DialectDenote SLLVM where
   denote
-  | udiv _ flag => fun ([x, y]ₕ) _ => ([·]ₕ) <$> LeanMLIR.SLLVM.udiv x y flag
-  | sdiv _ flag => fun ([x, y]ₕ) _ => ([·]ₕ) <$> LeanMLIR.SLLVM.sdiv x y flag
-  | urem _      => fun ([x, y]ₕ) _ => ([·]ₕ) <$> LeanMLIR.SLLVM.urem x y
-  | srem _      => fun ([x, y]ₕ) _ => ([·]ₕ) <$> LeanMLIR.SLLVM.srem x y
-  | op => fun args .nil =>
-    EffectKind.liftEffect (EffectKind.pure_le _) <|
+  | Op.udiv _ flag => fun ([x, y]ₕ) _ => ([·]ₕ) <$> SLLVM.udiv x y flag
+  | Op.sdiv _ flag => fun ([x, y]ₕ) _ => ([·]ₕ) <$> SLLVM.sdiv x y flag
+  | Op.urem _      => fun ([x, y]ₕ) _ => ([·]ₕ) <$> SLLVM.urem x y
+  | Op.srem _      => fun ([x, y]ₕ) _ => ([·]ₕ) <$> SLLVM.srem x y
+  | Op.arith op => fun args .nil => do
+    let x ← EffectKind.liftEffect (EffectKind.pure_le _) <|
+      let args := SLLVM.argsToLLVM args
       DialectDenote.denote (d := LLVM) op args .nil
-  -- ^^ For all other ops, just refer to the pure LLVM semantics
+      return x.map' SLLVM.Ty.arith (fun _ x => x)
+  -- ^^ For all other arithmetic ops, just refer to the pure LLVM semantics
+
+  | .ptradd   => fun ([p, x]ₕ) _  => ([·]ₕ) <$> SLLVM.ptradd p x
+  | .load w   => fun ([p]ₕ) _     => ([·]ₕ) <$> SLLVM.load p w
+  | .store _  => fun ([p, x]ₕ) _  => (fun _ => []ₕ) <$> SLLVM.store p x
+  | .free     => fun ([p]ₕ) _     => (fun _ => []ₕ) <$> SLLVM.free p
+
+/-! ### Printing -/
+section Print
+
+instance : ToString SLLVM.Ty where
+  toString := fun
+    | .arith ty => toString ty
+    | .ptr => "ptr"
+
+instance : ToString SLLVM.Op where
+  toString := fun
+    | .arith op => toString op
+    | .ptradd   => "ptradd"
+    | .load _   => "load"
+    | .store _  => "store"
+    | .free     => "free"
+
+instance : Repr SLLVM.Ty where
+  reprPrec ty _ := toString ty
+instance : Repr SLLVM.Op where
+  reprPrec op _ := toString op
+
+end Print
