SSA/Projects/SLLVM/Dialect/Refinement.lean
@@ -6,10 +6,40 @@ import SSA.Projects.SLLVM.Dialect.Base
 
 namespace LeanMLIR.SLLVM
 
-open InstCombine.LLVM.Ty (bitvec)
+
+open SLLVM.Ty in
+inductive Ty.IsRefinedBy : {t u : SLLVM.Ty} → ⟦t⟧ → ⟦u⟧ → Prop
+  | bitvec {w v} (x : LLVM.IntW w) (y : LLVM.IntW v) : x ⊑ y → @IsRefinedBy (bitvec _) (bitvec _) x y
+  | ptr (p q : SLLVM.Ptr) : p = q → @IsRefinedBy ptr ptr p q
 
 @[simp, simp_denote]
 instance instRefinement : DialectHRefinement SLLVM SLLVM where
   MonadIsRefinedBy := inferInstanceAs <| HRefinement (EffectM _) (EffectM _)
-  IsRefinedBy := @fun (bitvec _) (bitvec _) =>
-    inferInstanceAs <| HRefinement (LLVM.IntW _) (LLVM.IntW _)
+  IsRefinedBy := { IsRefinedBy := Ty.IsRefinedBy }
+
+/-! ## Simp Lemmas-/
+section Lemmas
+open HRefinement (IsRefinedBy)
+open Ty (bitvec ptr)
+
+@[simp, simp_denote, simp_sllvm] theorem bitvec_isRefinedBy_bitvec :
+    @Ty.IsRefinedBy (bitvec w) (bitvec v) x y ↔ @IsRefinedBy (LLVM.IntW w) (LLVM.IntW v) _ x y := by
+  constructor
+  · exact fun | (.bitvec _ _ h) => h
+  · apply Ty.IsRefinedBy.bitvec
+
+@[simp, simp_denote, simp_sllvm] theorem ptr_isRefinedBy_ptr :
+    @Ty.IsRefinedBy ptr ptr x y ↔ x = y := by
+  constructor
+  · exact fun | (.ptr _ _ h) => h
+  · apply Ty.IsRefinedBy.ptr
+
+@[simp, simp_denote, simp_sllvm] theorem not_bitvec_isRefinedBy_ptr :
+    ¬(@Ty.IsRefinedBy (bitvec w) ptr x y) := by
+  rintro ⟨⟩
+@[simp, simp_denote, simp_sllvm] theorem not_ptr_isRefinedBy_bitvec :
+    ¬(@Ty.IsRefinedBy ptr (bitvec w) x y) := by
+  rintro ⟨⟩
+
+
+end Lemmas
