SSA/Projects/SLLVM/Dialect/Parser.lean
@@ -23,12 +23,12 @@ instance : TransformTy SLLVM 0 where
   mkTy := mkTy
 
 
-def getOutputWidth (opStx : MLIR.AST.Op φ) (op : String) :
-    Except TransformError (Width φ) := do
+def getOutputWidth (opStx : MLIR.AST.Op 0) (op : String) :
+    Except TransformError Nat := do
   match opStx.res with
   | res::[] =>
     match res.2 with
-    | .int _ w => pure w
+    | .int _ (.concrete w) => pure w
     | _ => throw <| .generic s!"The operation {op} must output an integer type"
   | _ => throw <| .generic s!"The operation {op} must have a single output"
 
@@ -37,8 +37,9 @@ def getOutputWidth (opStx : MLIR.AST.Op φ) (op : String) :
 This relies on the fact that `bitvec _` is the only type currently modelled.
 In future, this might start throwing errors, if the type is not a bitvec.
 -/
-def getVarWidth {Γ : Ctxt SLLVM.Ty} : (Σ t, Γ.Var t) → Nat
-  | ⟨Ty.bitvec w, _⟩ => w
+def getIntWidth {Γ : Ctxt SLLVM.Ty} : (Σ t, Γ.Var t) → ReaderM Nat
+  | ⟨Ty.bitvec w, _⟩ => return w
+  | ⟨t, _⟩ => throw <| .generic s!"Expected type `bitvec _`, but found: {t}"
 
 def parseOverflowFlags (op : AST.Op 0) : ReaderM LLVM.NoWrapFlags :=
   match op.getAttr? "overflowFlags" with
@@ -54,7 +55,6 @@ def parseOverflowFlags (op : AST.Op 0) : ReaderM LLVM.NoWrapFlags :=
     | _ => throw <| .generic s!"Unrecognised overflow flag found: {MLIR.AST.docAttrVal y}. \
         We currently support nsw (no signed wrap) and nuw (no unsigned wrap)"
 
-open InstCombine (MOp) in
 instance : TransformExpr SLLVM 0 where
   mkExpr (Γ : Ctxt SLLVM.Ty) (opStx : MLIR.AST.Op 0) := do
   let args ← opStx.parseArgs Γ
@@ -63,56 +63,58 @@ instance : TransformExpr SLLVM 0 where
   let binW := do
   -- ^^ NOTE: `binW` is bound with := rather than ← on purpose, to ensure laziness
     let args ← args.assumeArity 2
-    return getVarWidth args[0]
+    getIntWidth args[0]
 
   /- `unW` is the (lazily computed) width, assuming an unary operation -/
   let unW := do
     let args ← args.assumeArity 1
-    return getVarWidth args[0]
+    getIntWidth args[0]
 
   let mkExprOf := opStx.mkExprOf (args? := args) Γ
   match opStx.name with
     -- Ternary Operations
     | "llvm.select" =>
         let args ← args.assumeArity 3
-        let w := getVarWidth args[1]
-        mkExprOf <| MOp.select w
+        let w ← getIntWidth args[1]
+        mkExprOf <| Op.select w
     -- Binary Operations
-    | "llvm.and"      => mkExprOf <| MOp.and (← binW)
-    | "llvm.or"       => mkExprOf <| MOp.or (← binW) ⟨opStx.hasAttr "isDisjoint"⟩
-    | "llvm.xor"      => mkExprOf <| MOp.xor (← binW)
-    | "llvm.urem"     => mkExprOf <| MOp.urem (← binW)
-    | "llvm.srem"     => mkExprOf <| MOp.srem (← binW)
-    | "llvm.lshr"     => mkExprOf <| MOp.lshr (← binW) ⟨opStx.hasAttr "isExact"⟩
-    | "llvm.ashr"     => mkExprOf <| MOp.ashr (← binW) ⟨opStx.hasAttr "isExact"⟩
-    | "llvm.sdiv"     => mkExprOf <| MOp.sdiv (← binW) ⟨opStx.hasAttr "isExact"⟩
-    | "llvm.udiv"     => mkExprOf <| MOp.udiv (← binW) ⟨opStx.hasAttr "isExact"⟩
-    | "llvm.shl"      => mkExprOf <| MOp.shl (← binW) (← parseOverflowFlags opStx)
-    | "llvm.add"      => mkExprOf <| MOp.add (← binW) (← parseOverflowFlags opStx)
-    | "llvm.mul"      => mkExprOf <| MOp.mul (← binW) (← parseOverflowFlags opStx)
-    | "llvm.sub"      => mkExprOf <| MOp.sub (← binW) (← parseOverflowFlags opStx)
-    | "llvm.icmp.eq"  => mkExprOf <| MOp.icmp .eq (← binW)
-    | "llvm.icmp.ne"  => mkExprOf <| MOp.icmp .ne (← binW)
-    | "llvm.icmp.ugt" => mkExprOf <| MOp.icmp .ugt (← binW)
-    | "llvm.icmp.uge" => mkExprOf <| MOp.icmp .uge (← binW)
-    | "llvm.icmp.ult" => mkExprOf <| MOp.icmp .ult (← binW)
-    | "llvm.icmp.ule" => mkExprOf <| MOp.icmp .ule (← binW)
-    | "llvm.icmp.sgt" => mkExprOf <| MOp.icmp .sgt (← binW)
-    | "llvm.icmp.sge" => mkExprOf <| MOp.icmp .sge (← binW)
-    | "llvm.icmp.slt" => mkExprOf <| MOp.icmp .slt (← binW)
-    | "llvm.icmp.sle" => mkExprOf <| MOp.icmp .sle (← binW)
+    | "llvm.and"      => mkExprOf <| Op.and (← binW)
+    | "llvm.or"       => mkExprOf <| Op.or (← binW) ⟨opStx.hasAttr "isDisjoint"⟩
+    | "llvm.xor"      => mkExprOf <| Op.xor (← binW)
+    | "llvm.urem"     => mkExprOf <| Op.urem (← binW)
+    | "llvm.srem"     => mkExprOf <| Op.srem (← binW)
+    | "llvm.lshr"     => mkExprOf <| Op.lshr (← binW) ⟨opStx.hasAttr "isExact"⟩
+    | "llvm.ashr"     => mkExprOf <| Op.ashr (← binW) ⟨opStx.hasAttr "isExact"⟩
+    | "llvm.sdiv"     => mkExprOf <| Op.sdiv (← binW) ⟨opStx.hasAttr "isExact"⟩
+    | "llvm.udiv"     => mkExprOf <| Op.udiv (← binW) ⟨opStx.hasAttr "isExact"⟩
+    | "llvm.shl"      => mkExprOf <| Op.shl (← binW) (← parseOverflowFlags opStx)
+    | "llvm.add"      => mkExprOf <| Op.add (← binW) (← parseOverflowFlags opStx)
+    | "llvm.mul"      => mkExprOf <| Op.mul (← binW) (← parseOverflowFlags opStx)
+    | "llvm.sub"      => mkExprOf <| Op.sub (← binW) (← parseOverflowFlags opStx)
+    | "llvm.icmp.eq"  => mkExprOf <| Op.icmp .eq (← binW)
+    | "llvm.icmp.ne"  => mkExprOf <| Op.icmp .ne (← binW)
+    | "llvm.icmp.ugt" => mkExprOf <| Op.icmp .ugt (← binW)
+    | "llvm.icmp.uge" => mkExprOf <| Op.icmp .uge (← binW)
+    | "llvm.icmp.ult" => mkExprOf <| Op.icmp .ult (← binW)
+    | "llvm.icmp.ule" => mkExprOf <| Op.icmp .ule (← binW)
+    | "llvm.icmp.sgt" => mkExprOf <| Op.icmp .sgt (← binW)
+    | "llvm.icmp.sge" => mkExprOf <| Op.icmp .sge (← binW)
+    | "llvm.icmp.slt" => mkExprOf <| Op.icmp .slt (← binW)
+    | "llvm.icmp.sle" => mkExprOf <| Op.icmp .sle (← binW)
     -- Unary Operations
-    | "llvm.not"   => mkExprOf <| MOp.not (← unW)
-    | "llvm.neg"   => mkExprOf <| MOp.neg (← unW)
-    | "llvm.copy"  => mkExprOf <| MOp.copy (← unW)
-    | "llvm.zext"  => mkExprOf <| MOp.zext (← unW) (← getOutputWidth opStx "zext") ⟨ opStx.hasAttr "nonNeg" ⟩
-    | "llvm.sext"  => mkExprOf <| MOp.sext (← unW) (← getOutputWidth opStx "sext")
-    | "llvm.trunc" => mkExprOf <| MOp.trunc (← unW) (← getOutputWidth opStx "trunc") (← parseOverflowFlags opStx)
+    | "llvm.not"   => mkExprOf <| Op.not (← unW)
+    | "llvm.neg"   => mkExprOf <| Op.neg (← unW)
+    | "llvm.copy"  => mkExprOf <| Op.copy (← unW)
+    | "llvm.zext"  => mkExprOf <| Op.zext (← unW) (← getOutputWidth opStx "zext") ⟨ opStx.hasAttr "nonNeg" ⟩
+    | "llvm.sext"  => mkExprOf <| Op.sext (← unW) (← getOutputWidth opStx "sext")
+    | "llvm.trunc" => mkExprOf <| Op.trunc (← unW) (← getOutputWidth opStx "trunc") (← parseOverflowFlags opStx)
     -- Constant
-    | "llvm.mlir.constant" =>
+    | "llvm.mlir.constant" => do
       let ⟨val, ty⟩ ← opStx.getIntAttr "value"
-      let opTy@(.bitvec w) ← mkTy ty
-      mkExprOf <| MOp.const w val
+      let opTy ← mkTy ty
+      let Ty.bitvec w := opTy
+        | throw <| .generic s!"Expected a `bitvec _`, but found: {opTy}"
+      mkExprOf <| Op.const w val
     -- Fallback
     | opName => throw <| .unsupportedOp opName
 
