SSA/Projects/SLLVM/Dialect/Semantics/Memory.lean
@@ -1,0 +1,55 @@
+import SSA.Core.Framework.Refinement
+import SSA.Projects.SLLVM.Tactic.SimpSet
+
+namespace LeanMLIR
+
+structure BlockId where
+  id : Nat
+  deriving DecidableEq, Hashable, Inhabited
+
+/-!
+**SIMPLIFICATION**
+We don't support storing poison, only fully-defined values!
+-/
+
+structure LiveBlock where
+  (length : Nat)
+  (bytes : BitVec (8 * length))
+
+inductive Block where
+  /-- A block of memory which was allocated and then freed. -/
+  | dead
+  /-- A live piece of memory (i.e., has been allocated and not yet freed). -/
+  | live (b : LiveBlock)
+
+structure MemoryState where
+  mem : Std.HashMap BlockId Block
+  nextFreeBlock : Nat
+  deriving Inhabited
+
+structure Pointer where
+  id : BlockId
+  /-- Offset in bytes -/
+  offset : BitVec 64
+  deriving Inhabited
+
+/-! ## Basic Definitions -/
+
+instance : GetElem? MemoryState BlockId Block (fun m i => i ∈ m.mem) where
+  getElem mem id h := mem.mem[id]
+  getElem? mem id  := mem.mem[id]?
+
+def LiveBlock.lengthInBits (b : LiveBlock) : Nat :=
+  8 * b.length
+
+def Pointer.offsetInBits (p : Pointer) : Nat :=
+  8 * p.offset.toNat
+
+/-! ## Refinement -/
+section Refinement
+
+instance : Refinement MemoryState where
+  IsRefinedBy s t := ∀ (id : BlockId),
+    s[id]? = t[id]?
+
+end Refinement
