SSA/Projects/SLLVM/Dialect/Semantics/MemorySemantics.lean
@@ -1,0 +1,128 @@
+/-
+Released under Apache 2.0 license as described in the file LICENSE.
+-/
+
+import SSA.Projects.SLLVM.Dialect.Semantics.EffectM
+import SSA.Projects.SLLVM.Dialect.Semantics.ArithSemantics
+import SSA.Projects.SLLVM.Tactic.SimpSet
+
+
+
+/-- `x.getOrUB` raises UB if `x` is poison. -/
+def PoisonOr.getOrUB  : PoisonOr α → LeanMLIR.EffectM α
+  | .value x => pure x
+  | .poison => .ub
+
+/-- `x.getOrUB` raises UB if `x` is `none` -/
+def Option.getOrUB : Option α → LeanMLIR.EffectM α
+  | .some x => pure x
+  | .none => .ub
+
+namespace LeanMLIR
+
+/-! ## Instructions -/
+namespace SLLVM
+open BitVec
+
+/--
+Return the block pointed to by `p`, or throw UB if this block
+- doesn't exists (i.e., hasn't been allocated yet), or
+- has been freed already
+-/
+def getLiveBlockOrUB (p : Pointer) : EffectM LiveBlock := do
+  let m ← getThe MemoryState
+  let some (.live block) := m[p.id]?
+    | .ub
+  return block
+
+/-- throw UB if `p` is true -/
+def throwUBIf (p : Prop) [Decidable p] : EffectM Unit :=
+  if p then .ub else pure ()
+
+
+/--
+`load p n` will load `n` bits from the location pointed to by `p`.
+
+Raises UB if:
+- `p` is poison
+- The block pointed to by `p.id` has not been allocated yet or has been freed already
+- The range of bits to be read is out of range of the block pointed to by `p.id`
+
+**SIMPLIFICATION**: we don't model alignment constraints at all
+-/
+def load (p : SLLVM.Ptr) (w : Nat) : EffectM (LLVM.IntW w) := do
+  let p ← p.getOrUB
+  let block ← getLiveBlockOrUB p
+  throwUBIf <| p.offsetInBits + w > block.lengthInBits
+  .value <| block.bytes.extractLsb' p.offsetInBits w
+
+/--
+`store p x` will store the value `x` at the location pointed to by `p`.
+
+Raises UB if:
+- `p` is poison
+- The block pointed to by `p.id` has not been allocated yet or has been freed already
+- The range of bits to be written is out of range of the block pointed to by `p.id`
+
+**SIMPLIFICATION**: we don't model alignment constraints at all
+-/
+def store (p : SLLVM.Ptr) (x : LLVM.IntW w) : EffectM Unit := do
+  let p ← p.getOrUB
+  let x ← x.getOrUB
+  let block ← getLiveBlockOrUB p
+  throwUBIf <| p.offsetInBits + w > block.lengthInBits
+  let bytes := block.bytes ||| (x.zeroExtend _ >>> p.offsetInBits)
+  modifyThe MemoryState fun m => { m with
+    mem := m.mem.insert p.id (.live { block with bytes })
+  }
+  return ()
+
+/--
+Free a block of memory
+
+Raises UB if:
+- `p` is poison
+- The block pointed to by `p.id` has not been allocated yet or has been freed already
+-/
+def free (p : SLLVM.Ptr) : EffectM Unit := do
+  let p ← p.getOrUB
+  let _ ← getLiveBlockOrUB p
+  modifyThe MemoryState fun m => { m with
+    mem := m.mem.insert p.id .dead
+  }
+
+/--
+Allocate a block of `n` *bytes* of memory, and return a pointer pointing to the
+start of the freshly allocated block.
+
+Raises UB if `n` is poison.
+-/
+def malloc (n : LLVM.IntW w) : EffectM SLLVM.Ptr := do
+  let n ← n.getOrUB
+  let p ← modifyGetThe MemoryState (allocate (8 * n.toNat))
+  .value p
+where
+  allocate (length : Nat) (m : MemoryState) : Pointer × MemoryState :=
+    let blockId := ⟨m.nextFreeBlock⟩
+    let nextFreeBlock := m.nextFreeBlock + 1
+    if blockId ∈ m.mem then
+      allocate length { m with nextFreeBlock }
+    else
+      let mem := m.mem.insert blockId (.live ⟨length, 0#_⟩)
+      ⟨ { id := blockId, offset := 0 },
+        { mem, nextFreeBlock }
+      ⟩
+  partial_fixpoint
+
+/-!
+TODO: Note that the above will deterministically pick the next available address.
+This is *not* actually the semantics we'd want. In reality, we probably need
+to say the an allocation non-deterministally picks any available address.
+Similarly, when definining the semantics of `split`, we'd probably want it to
+non-deterministally split up the available addresses between the two memory
+states.
+
+In any case, introducing non-determinism into `EffectM` and figuring this out
+exactly is left as work for a future PR. This is also why we don't have an
+`SLLVM.Op` for allocation yet.
+-/
